CoqCode/Auxiliaries.v
@@ -1,0 +1,13 @@
+Require Import Metalib.Metatheory.
+Require Import Language.
+
+Lemma value_to_term : forall (e : trm),
+    value e -> term e.
+Proof.
+  intros e Hval.
+  induction Hval.
+  - constructor.
+  - constructor.
+  - inversion H; subst. assumption.
+  - constructor. assumption. assumption.
+Qed.
